src/lowparse/LowParse.Spec.Enum.fst
@@ -422,3 +422,482 @@ let parse_maybe_total_enum_key_eq
 = parse_synth_eq p (maybe_total_enum_key_of_repr e) input;
   parse_synth_eq (parse_maybe_enum_key p e) (total_of_maybe_enum_key e) input;
   parse_synth_eq p (maybe_enum_key_of_repr e) input
+
+(* Destructors *)
+
+
+(* Universal destructor *)
+
+let r_reflexive_prop
+  (t: Type)
+  (r: (t -> t -> GTot Type0))
+: GTot Type0
+= forall (x: t) . r x x
+
+inline_for_extraction
+let r_reflexive_t
+  (t: Type)
+  (r: (t -> t -> GTot Type0))
+: Tot Type0
+= (x: t) -> Lemma (r x x)
+
+let r_reflexive_t_elim
+  (t: Type)
+  (r: (t -> t -> GTot Type0))
+  (phi: r_reflexive_t t r)
+: Lemma
+  (r_reflexive_prop t r)
+= Classical.forall_intro phi
+
+let r_transitive_prop
+  (t: Type)
+  (r: (t -> t -> GTot Type0))
+: GTot Type0
+= forall (x y z: t) . (r x y /\ r y z) ==> r x z
+
+inline_for_extraction
+let r_transitive_t
+  (t: Type)
+  (r: (t -> t -> GTot Type0))
+: Tot Type0
+= (x: t) -> (y: t) -> (z: t) -> Lemma ((r x y /\ r y z) ==> r x z)
+
+let r_transitive_t_elim
+  (t: Type)
+  (r: (t -> t -> GTot Type0))
+  (phi: r_transitive_t t r)
+: Lemma
+  (r_transitive_prop t r)
+= Classical.forall_intro_3 phi
+
+inline_for_extraction
+let if_combinator
+  (t: Type)
+  (eq: (t -> t -> GTot Type0))
+: Tot Type
+= (cond: bool) ->
+  (sv_true: (cond_true cond -> Tot t)) ->
+  (sv_false: (cond_false cond -> Tot t)) ->
+  Tot (y: t { eq y (if cond then sv_true () else sv_false ()) } )
+
+inline_for_extraction
+let default_if
+  (t: Type)
+: Tot (if_combinator t (eq2 #t))
+= fun
+  (cond: bool)
+  (s_true: (cond_true cond -> Tot t))
+  (s_false: (cond_false cond -> Tot t))
+-> (if cond
+  then s_true ()
+  else s_false ()) <: (y: t { y == (if cond then s_true () else s_false ()) } )
+
+let feq
+  (u v: Type)
+  (eq: (v -> v -> GTot Type0))
+  (f1 f2: (u -> Tot v))
+: GTot Type0
+= (forall (x: u) . eq (f1 x) (f2 x))
+
+inline_for_extraction
+let fif
+  (u v: Type)
+  (eq: (v -> v -> GTot Type0))
+  (ifc: if_combinator v eq)
+: Tot (if_combinator (u -> Tot v) (feq u v eq))
+= fun (cond: bool) (s_true: (cond_true cond -> u -> Tot v)) (s_false: (cond_false cond -> u -> Tot v)) (x: u) ->
+    ifc
+      cond
+      (fun h -> s_true () x)
+      (fun h -> s_false () x)
+
+inline_for_extraction
+let enum_destr_t
+  (t: Type)
+  (#key #repr: eqtype)  
+  (e: enum key repr)
+: Tot Type
+= (eq: (t -> t -> GTot Type0)) ->
+  (ift: if_combinator t eq) ->
+  (eq_refl: r_reflexive_t _ eq) ->
+  (eq_trans: r_transitive_t _ eq) ->
+  (f: ((x: enum_key e) -> Tot t)) ->
+  (x: enum_key e) ->
+  Tot (y: t { eq y (f x) } )
+
+inline_for_extraction
+let enum_tail'
+  (#key #repr: eqtype)
+  (e: enum key repr)
+: Pure (enum key repr)
+  (requires True)
+  (ensures (fun y -> Cons? e ==> (let (_ :: y') = e in y == y')))
+= match e with _ :: y -> y | _ -> []
+
+inline_for_extraction
+let enum_tail
+  (#key #repr: eqtype)
+  (e: enum key repr)
+: Tot (enum key repr)
+= enum_tail' e
+
+inline_for_extraction
+let enum_destr_cons
+  (t: Type)
+  (#key #repr: eqtype)
+  (e: enum key repr)
+  (g: enum_destr_t t (enum_tail' e))
+: Pure (enum_destr_t t e)
+  (requires (Cons? e))
+  (ensures (fun _ -> True))
+= fun (eq: (t -> t -> GTot Type0)) (ift: if_combinator t eq) (eq_refl: r_reflexive_t _ eq) (eq_trans: r_transitive_t _ eq) ->
+  [@inline_let]
+  let _ = r_reflexive_t_elim _ _ eq_refl in
+  [@inline_let]
+  let _ = r_transitive_t_elim _ _ eq_trans in
+  (fun (e' : list (key * repr) { e' == e } ) -> match e' with
+     | (k, _) :: _ ->
+     (fun (f: (enum_key e -> Tot t)) (x: enum_key e) -> ((
+       [@inline_let]
+       let f' : (enum_key (enum_tail' e) -> Tot t) =
+         (fun (x' : enum_key (enum_tail' e)) ->
+           [@inline_let]
+           let (x_ : enum_key e) = (x' <: key) in
+           f x_
+         )
+       in
+       [@inline_let]
+       let (y: t) =
+       ift
+         ((k <: key) = x)
+         (fun h -> f k)
+         (fun h ->
+           [@inline_let]
+           let x' : enum_key (enum_tail' e) = (x <: key) in
+           (g eq ift eq_refl eq_trans f' x' <: t))
+       in
+       y
+     ) <: (y: t { eq y (f x) } )))
+  ) e
+
+inline_for_extraction
+let enum_destr_cons'
+  (t: Type)
+  (key repr: eqtype)
+  (e: enum key repr)
+  (u: unit { Cons? e } )
+  (g: enum_destr_t t (enum_tail e))
+: Tot (enum_destr_t t e)
+= enum_destr_cons t e g
+
+inline_for_extraction
+let enum_destr_cons_nil
+  (t: Type)
+  (#key #repr: eqtype)
+  (e: enum key repr)
+: Pure (enum_destr_t t e)
+  (requires (Cons? e /\ Nil? (enum_tail' e)))
+  (ensures (fun _ -> True))
+= fun (eq: (t -> t -> GTot Type0)) (ift: if_combinator t eq) (eq_refl: r_reflexive_t _ eq) (eq_trans: r_transitive_t _ eq) ->
+  [@inline_let]
+  let _ = r_reflexive_t_elim _ _ eq_refl in
+  (fun (e' : list (key * repr) { e' == e } ) -> match e' with
+     | (k, _) :: _ ->
+     (fun (f: (enum_key e -> Tot t)) (x: enum_key e) -> ((
+       f k
+     ) <: (y: t { eq y (f x) } )))
+  ) e
+
+inline_for_extraction
+let enum_destr_cons_nil'
+  (t: Type)
+  (key repr: eqtype)
+  (e: enum key repr)
+  (u1: unit { Cons? e } )
+  (u2: unit { Nil? (enum_tail e) } )
+: Tot (enum_destr_t t e)
+= enum_destr_cons_nil t e
+
+(* Dependent destructor *)
+
+inline_for_extraction
+let dep_enum_destr
+  (#key #repr: eqtype)
+  (e: enum key repr)
+  (v: (enum_key e -> Tot Type))
+: Tot Type
+= (v_eq: ((k: enum_key e) -> v k -> v k -> GTot Type0)) ->
+  (v_if: ((k: enum_key e) -> Tot (if_combinator (v k) (v_eq k)))) ->
+  (v_eq_refl: ((k: enum_key e) -> Tot (r_reflexive_t _ (v_eq k)))) ->
+  (v_eq_trans: ((k: enum_key e) -> Tot (r_transitive_t _ (v_eq k)))) ->
+  (f: ((k: enum_key e) -> Tot (v k))) ->
+  (k: enum_key e) ->
+  Tot (y: v k { v_eq k y (f k) } )
+
+module L = FStar.List.Tot
+
+inline_for_extraction
+let dep_enum_destr_cons
+  (#key #repr: eqtype)
+  (e: enum key repr)
+  (u: squash (Cons? e))
+  (v: (enum_key e -> Tot Type))
+  (destr: dep_enum_destr (enum_tail e) (fun (k' : enum_key (enum_tail e)) -> v (k' <: key)))
+: Tot (dep_enum_destr e v)
+= match e with
+  | ((k, _) :: _) ->
+    fun
+    (v_eq: ((k: enum_key e) -> v k -> v k -> GTot Type0))
+    (v_if: ((k: enum_key e) -> Tot (if_combinator (v k) (v_eq k))))
+    (v_eq_refl: ((k: enum_key e) -> Tot (r_reflexive_t _ (v_eq k))))
+    (v_eq_trans: ((k: enum_key e) -> Tot (r_transitive_t _ (v_eq k))))
+    (f: ((k: enum_key e) -> Tot (v k)))
+    (k' : enum_key e) ->
+    [@inline_let]
+    let _ = r_reflexive_t_elim (v k') (v_eq k') (v_eq_refl k') in
+    [@inline_let]
+    let _ = r_transitive_t_elim (v k') (v_eq k') (v_eq_trans k') in  
+    [@inline_let]
+    let y : v k' =
+      v_if k' (k = k') (fun _ ->
+        [@inline_let]
+        let y : v k' = f k in
+        y
+      ) (fun _ ->
+        [@inline_let]
+        let v' (k: enum_key (enum_tail e)) : Tot Type = v (k <: key) in
+        [@inline_let]
+        let v'_eq (k: enum_key (enum_tail e)) : Tot (v' k -> v' k -> GTot Type0) = v_eq (k <: key) in
+        [@inline_let]
+        let v'_if (k: enum_key (enum_tail e)) : Tot (if_combinator (v' k) (v'_eq k)) = v_if (k <: key) in
+        [@inline_let]
+        let v'_eq_refl (k: enum_key (enum_tail e)) : Tot (r_reflexive_t _ (v'_eq k)) = v_eq_refl (k <: key) in
+        [@inline_let]
+        let v'_eq_trans (k: enum_key (enum_tail e)) : Tot (r_transitive_t _ (v'_eq k)) = v_eq_trans (k <: key) in
+        [@inline_let]
+        let f' (k: enum_key (enum_tail e)) : Tot (v' k) = f (k <: key) in
+        [@inline_let]
+        let k' : key = k' in
+        assert (k' <> k);
+        assert (L.mem k' (L.map fst (enum_tail e)));
+        [@inline_let]
+        let (y: v' k') =
+          destr v'_eq v'_if v'_eq_refl v'_eq_trans f' k'
+        in
+        y
+      )
+    in
+    (y <: (y: v k' { v_eq k' y (f k') } ))
+
+inline_for_extraction
+let dep_enum_destr_cons_nil
+  (#key #repr: eqtype)
+  (e: enum key repr)
+  (u: squash (Cons? e /\ Nil? (enum_tail e)))
+  (v: (enum_key e -> Tot Type))
+: Tot (dep_enum_destr e v)
+= match e with
+  | ((k, _) :: _) ->
+    fun
+    (v_eq: ((k: enum_key e) -> v k -> v k -> GTot Type0))
+    (v_if: ((k: enum_key e) -> Tot (if_combinator (v k) (v_eq k))))
+    (v_eq_refl: ((k: enum_key e) -> Tot (r_reflexive_t _ (v_eq k))))
+    (v_eq_trans: ((k: enum_key e) -> Tot (r_transitive_t _ (v_eq k))))
+    (f: ((k: enum_key e) -> Tot (v k)))
+    (k' : enum_key e) ->
+    [@inline_let]
+    let _ = r_reflexive_t_elim (v k') (v_eq k') (v_eq_refl k') in
+    [@inline_let]
+    let _ = r_transitive_t_elim (v k') (v_eq k') (v_eq_trans k') in  
+    [@inline_let]
+    let y : v k' = f k in
+    (y <: (y: v k' { v_eq k' y (f k') } ))
+
+(* Destructor from the representation *)
+
+
+let maybe_enum_key_of_repr_not_in (#key #repr: eqtype) (e: enum key repr) (l: list (key * repr)) (x: repr) : GTot Type0 =
+  (~ (L.mem x (L.map snd l)))
+
+let list_rev_cons
+  (#t: Type)
+  (a: t)
+  (q: list t)
+: Lemma
+  (L.rev (a :: q) == L.rev q `L.append` [a])
+= L.rev_rev' (a :: q);
+  L.rev_rev' q
+
+let list_append_rev_cons (#t: Type) (l1: list t) (x: t) (l2: list t) : Lemma
+  (L.append (L.rev l1) (x :: l2) == L.append (L.rev (x :: l1)) l2)
+= list_rev_cons x l1;
+  L.append_assoc (L.rev l1) [x] l2
+
+let rec assoc_append_flip_l_intro
+  (#key #repr: eqtype)
+  (l1 l2: list (key * repr))
+  (y: repr)
+  (x: key)
+: Lemma
+  (requires (L.noRepeats (L.map snd (L.append l1 l2)) /\ L.assoc y (L.map flip l2) == Some x))
+  (ensures (L.assoc y (L.map flip (l1 `L.append` l2)) == Some x))
+= match l1 with
+  | [] -> ()
+  | (_, r') :: q ->
+    L.assoc_mem y (L.map flip l2);
+    map_fst_flip l2;
+    L.map_append snd l1 l2;
+    L.noRepeats_append_elim (L.map snd l1) (L.map snd l2);
+    assoc_append_flip_l_intro q l2 y x
+
+inline_for_extraction
+let maybe_enum_destr_t'
+  (t: Type)
+  (#key #repr: eqtype)  
+  (e: enum key repr)
+  (l1 l2: list (key * repr))
+  (u1: squash (e == L.append (L.rev l1) l2))
+: Tot Type
+= (eq: (t -> t -> GTot Type0)) ->
+  (ift: if_combinator t eq) ->
+  (eq_refl: r_reflexive_t _ eq) ->
+  (eq_trans: r_transitive_t _ eq) ->
+  (f: ((x: maybe_enum_key e) -> Tot t)) ->
+  (x: repr { maybe_enum_key_of_repr_not_in e l1 x } ) ->
+  Tot (y: t { eq y (f (maybe_enum_key_of_repr e x)) } )
+
+inline_for_extraction
+let maybe_enum_destr_t
+  (t: Type)
+  (#key #repr: eqtype)  
+  (e: enum key repr)
+: Tot Type
+= (eq: (t -> t -> GTot Type0)) ->
+  (ift: if_combinator t eq) ->
+  (eq_refl: r_reflexive_t _ eq) ->
+  (eq_trans: r_transitive_t _ eq) ->
+  (f: ((x: maybe_enum_key e) -> Tot t)) ->
+  (x: repr) ->
+  Tot (y: t { eq y (f (maybe_enum_key_of_repr e x)) } )
+
+inline_for_extraction
+let destr_maybe_total_enum_repr
+  (#t: Type)
+  (#key #repr: eqtype)
+  (e: total_enum key repr)
+  (destr: maybe_enum_destr_t t e)
+  (eq: (t -> t -> GTot Type0))
+  (ift: if_combinator t eq)
+  (eq_refl: r_reflexive_t _ eq)
+  (eq_trans: r_transitive_t _ eq)
+  (f: ((x: maybe_total_enum_key e) -> Tot t))
+  (x: repr)
+: Tot (y: t { eq y (f (maybe_total_enum_key_of_repr e x)) } )
+= destr eq ift eq_refl eq_trans (fun y -> f (total_of_maybe_enum_key e y)) x
+
+inline_for_extraction
+let maybe_enum_destr_t_intro
+  (t: Type)
+  (#key #repr: eqtype)  
+  (e: enum key repr)
+  (f: maybe_enum_destr_t' t e [] e ())
+: Tot (maybe_enum_destr_t t e)
+= f
+
+let maybe_enum_key_of_repr_not_in_cons
+  (#key #repr: eqtype)
+  (e: enum key repr)
+  (k: key)
+  (r: repr)
+  (l: list (key * repr))
+  (x: repr)
+: Lemma
+  (requires (maybe_enum_key_of_repr_not_in e l x /\ x <> r))
+  (ensures (maybe_enum_key_of_repr_not_in e ((k, r) :: l) x))
+= ()
+
+inline_for_extraction
+let list_hd
+  (#t: Type)
+  (l: list t { Cons? l } )
+= match l with
+  | a :: _ -> a
+
+inline_for_extraction
+let list_tl
+  (#t: Type)
+  (l: list t { Cons? l } )
+= match l with
+  | _ :: q -> q
+
+inline_for_extraction
+let maybe_enum_destr_cons
+  (t: Type)
+  (#key #repr: eqtype)
+  (e: enum key repr)
+  (l1: list (key * repr))
+  (l2: list (key * repr))
+  (u1: squash (Cons? l2 /\ e == L.append (L.rev l1) l2))
+  (g: (maybe_enum_destr_t' t e (list_hd l2 :: l1) (list_tl l2) (list_append_rev_cons l1 (list_hd l2) (list_tl l2))))
+: Tot (maybe_enum_destr_t' t e l1 l2 u1)
+= fun (eq: (t -> t -> GTot Type0)) (ift: if_combinator t eq) (eq_refl: r_reflexive_t _ eq) (eq_trans: r_transitive_t _ eq) (f: (maybe_enum_key e -> Tot t)) ->
+  [@inline_let]
+  let _ = r_reflexive_t_elim _ _ eq_refl in
+  [@inline_let]
+  let _ = r_transitive_t_elim _ _ eq_trans in
+  match list_hd l2 with
+  | (k, r) ->
+  [@inline_let]
+  let _ : squash (L.mem k (L.map fst e)) =
+    L.append_mem (L.map fst (L.rev l1)) (L.map fst l2) k;
+    L.map_append fst (L.rev l1) (l2);
+    ()
+  in
+  [@inline_let]
+  let (_ : squash (maybe_enum_key_of_repr e r == Known k)) =
+    L.append_mem (L.map snd (L.rev l1)) (L.map snd (l2)) r;
+    L.map_append snd (L.rev l1) (l2);
+    assoc_append_flip_l_intro (L.rev l1) (l2) r k;
+    ()
+  in
+  fun (x: repr { maybe_enum_key_of_repr_not_in e l1 x } ) -> ((
+    ift
+      (x = r)
+      (fun h -> f (Known k))
+      (fun h -> g eq ift eq_refl eq_trans f x)
+  ) <: (y: t { eq y (f (maybe_enum_key_of_repr e x)) } ))
+
+let rec list_rev_map
+  (#t1 #t2: Type)
+  (f: t1 -> Tot t2)
+  (l: list t1)
+: Lemma
+  (L.rev (L.map f l) == L.map f (L.rev l))
+= match l with
+  | [] -> ()
+  | a :: q ->
+    list_rev_cons a q;
+    list_rev_cons (f a) (L.map f q);
+    list_rev_map f q;
+    L.map_append f (L.rev q) [a]
+
+inline_for_extraction
+let maybe_enum_destr_nil
+  (t: Type)
+  (#key #repr: eqtype)
+  (e: enum key repr)
+  (l1: list (key * repr))
+  (l2: list (key * repr))
+  (u1: squash (Nil? l2 /\ e == L.append (L.rev l1) []))
+: Tot (maybe_enum_destr_t' t e l1 l2 u1)
+= fun (eq: (t -> t -> GTot Type0)) (ift: if_combinator t eq) (eq_refl: r_reflexive_t _ eq) (eq_trans: r_transitive_t _ eq) (f: (maybe_enum_key e -> Tot t)) ->
+  [@inline_let]
+  let _ = r_reflexive_t_elim _ _ eq_refl in
+  [@inline_let]
+  let _ = r_transitive_t_elim _ _ eq_trans in
+  fun (x: repr { maybe_enum_key_of_repr_not_in e l1 x } ) -> ((
+    L.append_l_nil (L.rev l1);
+    list_rev_map snd l1;
+    L.rev_mem (L.map snd l1) x;
+    f (Unknown x)
+  ) <: (y: t { eq y (f (maybe_enum_key_of_repr e x)) } ))
